Ch4.v
@@ -1,0 +1,76 @@
+Set Implicit Arguments.
+Unset Strict Implicit.
+Unset Printing Implicit Defensive.
+From Coq Require Import ssreflect.
+
+Module Ch4.
+  Inductive term : Type :=
+  | T_true
+  | T_false
+  | T_cond (cond t1 t2 : term)
+  | T_zero
+  | T_succ (n : term)
+  | T_pred (n : term)
+  | T_iszero (n : term).
+
+  Fixpoint isnumericval t :=
+    match t with
+    | T_zero => true
+    | T_succ t' => isnumericval t'
+    | _ => false
+    end.
+
+  Compute (isnumericval T_true).
+  Compute (isnumericval T_zero).
+  Compute (isnumericval (T_succ T_true)).
+  Compute (isnumericval (T_pred T_zero)).
+  Compute (isnumericval (T_succ T_zero)).
+
+  Fixpoint isval t :=
+    match t with
+    | T_true | T_false => true
+    | t' => isnumericval t'
+    end.
+
+  Compute (isval (T_succ T_zero)).
+  Compute (isval (T_succ (T_succ T_zero))).
+  Compute (isval (T_pred (T_succ T_zero))).
+  Compute (isval (T_pred (T_iszero T_zero))).
+
+  (* Single-step evaluation (partial function) *)
+
+  Fixpoint eval1 t :=
+    match t with
+    | T_cond T_true t _ =>
+      Some t
+    | T_cond T_false _ t =>
+      Some t
+    | T_cond cond t1 t2 =>
+      match eval1 cond with
+      | Some cond' => Some (T_cond cond' t1 t2)
+      | None => None
+      end
+    | T_succ t' =>
+      match eval1 t' with
+      | Some v => Some (T_succ v)
+      | None => None
+      end
+    | T_pred T_zero =>
+      Some T_zero
+    | T_pred t' =>
+      if t' is T_succ t'' then
+        if isnumericval t'' then (Some t'') else None
+      else
+        if eval1 t' is Some v then Some (T_pred v) else None
+    | T_iszero T_zero =>
+      Some T_true
+    | T_iszero t' =>
+      if t' is T_succ t'' then
+        if isnumericval t'' then (Some T_false) else None
+      else
+        if eval1 t' is Some v then (Some (T_iszero v)) else None
+    | _ =>
+      None
+    end.
+
+End Ch4.
